Some WF properties. Currently stuck at validsize_children.

examples/containers/theories/SetProofs.v
@@ -21,27 +21,79 @@ Module Foo (E : OrderedType) : WSfun(E).
     end.
   
   Local Instance Ord_t : GHC.Base.Ord E.t := GHC.Base.ord_default compare.
-
+  
   Module OrdFacts := OrderedTypeFacts(E).
 
   Definition elt := E.t.
   
   (* Well-formedness *)
-  Definition WF (s : Set_ elt) := True. (* TODO. maybe simply [valid s = true]? *)
+  Definition WF (s : Set_ elt) := valid s.
+  (* Will it be easier for proof if [WF] is an inductive definition? *)
   Definition t := {s : Set_ elt | WF s}.
   Definition pack (s : Set_ elt) (H : WF s): t := exist _ s H.
 
+  Lemma balanced_children : forall {a} (s1 s2 : Set_ a) l e,
+      balanced (Bin l e s1 s2) -> balanced s1 /\ balanced s2.
+  Proof. split; simpl in H; move: H; case: and3P=>//; elim; done. Qed.
+
+  Lemma ordered_children : forall {a} `{Eq_ a} `{Ord a} (s1 s2 : Set_ a) l e,
+      ordered (Bin l e s1 s2) -> ordered s1 /\ ordered s2.
+  Proof.
+    split; unfold ordered in *; move: H2; case: and4P=>//; elim; intros.
+    - remember (const true) as ct. rewrite {2}[ct] Heqct.
+      clear H5; clear Heqct; clear H2; clear H3. generalize dependent ct.
+      induction s1=>//. intros. move: H4; case: and4P=>//; elim.
+      intros. apply /and4P; split=>//. apply IHs1_2; auto.
+    - remember (const true) as ct. rewrite {1}[ct] Heqct.
+      clear H4; clear Heqct; clear H2; clear H3. generalize dependent ct.
+      induction s2=>//. intros. move: H5; case: and4P=>//; elim.
+      intros. apply /and4P; split=>//. apply IHs2_1; auto.
+  Qed.
+
+  Lemma validsize_children : forall {a} (s1 s2 : Set_ a) l e,
+      validsize (Bin l e s1 s2) -> validsize s1 /\ validsize s2.
+  Proof.
+    split; move: H; rewrite /validsize=>H;
+      remember (fix realsize (t' : Set_ a) : option Size :=
+                  match t' with
+                  | Bin sz _ l r =>
+                    match realsize l with
+                    | Some n =>
+                      match realsize r with
+                      | Some m =>
+                        if _GHC.Base.==_ (n + m + 1)%Z sz
+                        then Some sz
+                        else None
+                      | None => None
+                      end
+                    | None => None
+                    end
+                  | Tip => Some 0%Z
+                  end) as f; move: H; rewrite -Heqf.
+  (* I'm stuck here *)
+  Admitted.
+      
+  Lemma WF_children : forall s1 s2 l e, WF (Bin l e s1 s2) -> WF s1 /\ WF s2.
+  Proof.
+    rewrite /WF /valid. move=>s1 s2 l e. case: and3P=>//.
+    elim; move=>Hb Ho Hv H; clear H. 
+    split; apply /and3P; split;
+      apply balanced_children in Hb;
+      apply ordered_children in Ho;
+      apply validsize_children in Hv; intuition.
+  Qed.
+  
   Definition In x (s' : t) := match s' with exist s P =>
      member x s = true
      end.
-
+  
   Definition Equal s s' := forall a : elt, In a s <-> In a s'.
   Definition Subset s s' := forall a : elt, In a s -> In a s'.
   Definition Empty s := forall a : elt, ~ In a s.
   Definition For_all (P : elt -> Prop) s := forall x, In x s -> P x.
   Definition Exists (P : elt -> Prop) s := exists x, In x s /\ P x.
 
-  Definition empty : t := pack empty I.
+  Definition empty : t := pack empty eq_refl.
   Definition is_empty : t -> bool := fun s' => match s' with exist s _ =>
      null s end.
   Definition mem : elt -> t -> bool := fun e s' => match s' with exist s _ =>
@@ -85,22 +137,22 @@ Module Foo (E : OrderedType) : WSfun(E).
     (* LY: Surely this can be simplified? *)
     unfold In; destruct s as [s']; induction s'; auto. intros.
     simpl in H0; destruct (Base.compare x a) eqn:Hcomp;
-      vm_compute in Hcomp; destruct (E.compare x a);
+      vm_compute in Hcomp; destruct (E.compare x a) as [HL | HE | HG];
         inversion Hcomp; clear Hcomp.
-    - apply E.eq_sym in H. apply (E.eq_trans H) in e.
-      apply OrdFacts.elim_compare_eq in e; destruct e as [? Heq].
+    - apply E.eq_sym in H. apply (E.eq_trans H) in HE.
+      apply OrdFacts.elim_compare_eq in HE; destruct HE as [? Heq].
       simpl. vm_compute. rewrite Heq; auto.
-    - apply (OrdFacts.eq_lt (E.eq_sym H)) in l.
-      apply OrdFacts.elim_compare_lt in l; destruct l as [? Hlt]. simpl.
+    - apply (OrdFacts.eq_lt (E.eq_sym H)) in HL.
+      apply OrdFacts.elim_compare_lt in HL; destruct HL as [? Hlt]. simpl.
       assert (Hcomp: Base.compare y a = Lt).
       { vm_compute. rewrite Hlt; auto. }
-      rewrite Hcomp. eauto.
+      rewrite Hcomp. apply WF_children in i; destruct i. eauto.
     - assert (Heq: E.eq x y) by apply H.
-      apply (OrdFacts.lt_eq l) in H.
+      apply (OrdFacts.lt_eq HG) in H.
       apply OrdFacts.elim_compare_gt in H; destruct H as [? Hgt]. simpl.
       assert (Hcomp: Base.compare y a = Gt).
       { vm_compute. rewrite Hgt; auto. }
-      rewrite Hcomp. eauto.
+      rewrite Hcomp. apply WF_children in i; destruct i. eauto.
   Qed.
       
   Lemma eq_refl : forall s : t, eq s s.
@@ -129,7 +181,7 @@ Module Foo (E : OrderedType) : WSfun(E).
   
   Lemma empty_1 : Empty empty.
   Proof. unfold Empty; intros a H. inversion H. Qed.
-    
+  
   Lemma is_empty_1 : forall s : t, Empty s -> is_empty s = true.
   Proof.
     unfold Empty; unfold In. destruct s; destruct x; auto.
